add replace_utf8_encoded

eval/send_packet.py
@@ -2,7 +2,7 @@ import socket
 
 def get_topic_length(topic_name_length):
     hex_str = '{0:04x}'.format(topic_name_length)
-    return hex_str[0:2] + ' ' + hex_str[2:4]
+    return hex_str[0:2] + hex_str[2:4]
 
 def encode_remaining_length(remaining_length):
     remaining_length_hex_str = ''
@@ -11,7 +11,7 @@ def encode_remaining_length(remaining_length):
         remaining_length //= 128
         if remaining_length > 0:
             d |= 128
-        remaining_length_hex_str += '{0:02x} '.format(d & 255)
+        remaining_length_hex_str += '{0:02x}'.format(d & 255)
         if remaining_length == 0:
             break
     return remaining_length_hex_str
@@ -27,7 +27,7 @@ tcp_client.connect((target_ip,target_port))
 tcp_client.send(b"\x10\x10\x00\x04\x4d\x51\x54\x54\x05\x02\x00\x3c\x03\x21\x00\x14\x00\x00")
 
 res = tcp_client.recv(buffer_size)
-print('Connect ACK:', res)
+# print('Connect ACK:', res)
 
 topic_name = 'example/topic'
 topic_name_length = len(topic_name)
@@ -35,13 +35,13 @@ topic_name_length = len(topic_name)
 payload = 'Hello MQTT!'
 payload_length = len(payload)
 
-# print(encode_remaining_length(topic_name_length + payload_length + 3))
 data = '30{}{}{}00{}'.format(
     encode_remaining_length(topic_name_length + payload_length + 3),
     get_topic_length(topic_name_length),
-    topic_name,
-    payload
+    topic_name.encode('utf-8', 'replace').hex(),
+    payload.encode('utf-8', 'replace').hex()
 )
-tcp_client.send(b"\x30\x30\x00\x0D\x65\x78\x61\x6D\x70\x6C\x65\x2F\x74\x6F\x70\x69\x63\x00\x68\x65\x6C\x6C\x6F\x20\x6D\x71\x74\x74\x21\x20\xE3\x81\x93\xE3\x82\x93\xE3\x81\xAB\xE3\x81\xA1\xE3\x81\xAF\x4D\x51\x54\x54\x21")
+
+tcp_client.send(bytearray.fromhex(data))
 
 tcp_client.send(b"\xe0\x00")
